Hashed El Gamal ported over. No abstract proof steps.

examples/hashed_elgamal.ec
@@ -3,358 +3,355 @@ require import Real.
 require import FMap. 
 require import FSet.
 require import CDH.
-require Logic.
-require AWord.
-require RandOrcl.
-require PKE.
+require (*--*) AWord.
+require (*--*) ROM.
+require (*--*) PKE.
 
-import OptionGet.
+(* The type of plaintexts: bitstrings of length k *)
+type bits.
+op k: int.
+op uniform: bits distr.
 
+clone import AWord as Bitstring with
+  type word <- bits,
+  op length <- k,
+  op Dword.dword <- uniform.
 
-const k : int.
+(* Upper bound on the number of calls to H *)
+op qH: int.
+axiom qH_pos: 0 < qH.
 
-clone AWord as Bitstring with op length = k.
-
-type bitstring = Bitstring.word.
-
-const qH : int.
-
-axiom qH_pos : 0 < qH.
-
-clone Set_CDH as SCDH with op n = qH.
+(* Assumption *)
+clone Set_CDH as SCDH with
+  op n <- qH.
 
 import Group.
 
 type pkey       = group.
 type skey       = int.
-type plaintext  = bitstring.
-type ciphertext = group * bitstring.
+type plaintext  = bits.
+type ciphertext = group * bits.
 
-op (^^) : bitstring -> bitstring -> bitstring = Bitstring.(^).
+op (^^): bits -> bits -> bits = (^)%Bitstring.
 
 clone import PKE as PKE_ with
-  type pkey = pkey,
-  type skey = skey,
-  type plaintext = plaintext,
-  type ciphertext = ciphertext. 
+  type pkey <- pkey,
+  type skey <- skey,
+  type plaintext <- plaintext,
+  type ciphertext <- ciphertext. 
 
 module type Hash = {
-  fun init() : unit
-  fun hash(x:group) : bitstring
+  proc init(): unit
+  proc hash(x:group): bits
 }.
 
-module Hashed_ElGamal (H:Hash) : Scheme = {
-  fun kg() : pkey * skey = {
-    var sk : int;
+module Hashed_ElGamal (H:Hash): Scheme = {
+  proc kg(): pkey * skey = {
+    var sk;
+
     H.init();
     sk = $[0..q-1];
     return (g ^ sk, sk);   
   }
 
-  fun enc(pk:pkey, m:plaintext) : ciphertext = {
-    var y : int;
-    var h : plaintext;
+  proc enc(pk:pkey, m:plaintext): ciphertext = {
+    var y, h;
+
     y = $[0..q-1];
     h = H.hash(pk ^ y);
     return (g ^ y, h ^^ m);
   }
 
-  fun dec(sk:skey, c:ciphertext) : plaintext option = {
-    var gy : group;
-    var h, hm : bitstring;
+  proc dec(sk:skey, c:ciphertext): plaintext option = {
+    var gy, h, hm;
+
     (gy, hm) = c; 
     h = H.hash(gy ^ sk);
     return Option.Some (h ^^ hm); 
   }
 }.
 
-op uniform : bitstring distr = Bitstring.Dword.dword.
+clone import ROM.Lazy as RandOrcl_group with 
+  type from  <- group,
+  type to    <- bits,
+  op dsample <- fun (x:group), uniform.
+import Types.
 
-clone import RandOrcl as RandOrcl_group with 
-  type from = group,
-  type to = bitstring,
-  op dsample = uniform,
-  op qO = qH,
-  op default = Bitstring.zeros.
-
-import ROM.
-import WRO_Set.
-
-(* ROM Adversary *)
-
-
+(* Adversary Definitions *)
 module type Adversary (O:ARO) = {
-  fun choose(pk:pkey)     : plaintext * plaintext {* O.o}
-  fun guess(c:ciphertext) : bool
+  proc choose(pk:pkey)    : plaintext * plaintext
+  proc guess(c:ciphertext): bool
 }.
 
-module AO = ARO(RO).
+module Bounder(A:Adversary,O:ARO) = {
+  module ARO = {
+    var qs:group set
 
-module H : Hash = {
-  fun init() : unit = { AO.init(); }
-  fun hash(x:group) : bitstring = { var y : bitstring; y = RO.o(x); return y; }
+    proc o(x:group): bits = {
+      var r = witness;
+
+      if (card qs < qH) {
+        r  = O.o(x);
+        qs = add x qs;
+      }
+      return r;
+    }
+  }
+
+  module A' = A(ARO)
+
+  proc choose = A'.choose
+  proc guess  = A'.guess
 }.
 
+(* Specializing and merging the hash function *)
+module H:Hash = {
+  proc init(): unit = { RO.init(); Bounder.ARO.qs = FSet.empty; }
+  proc hash(x:group): bits = { var y; y = RO.o(x); return y; }
+}.
+
+(* The initial scheme *)
 module S = Hashed_ElGamal(H).
 
+(* Correctness result *)
+hoare Correctness: Correctness(S).main: true ==> res.
+proof. by proc; inline *; auto; progress; smt. qed.
+
+(* The reduction *)
+module SCDH_from_CPA(A:Adversary,O:ARO): SCDH.Adversary = {
+  module BA = Bounder(A,O)
+
+  proc solve(gx:group, gy:group): group set = {
+    var m0, m1, h, b';
+
+    H.init();
+    (m0,m1)  = BA.choose(gx);
+    h        = $uniform;
+    b'       = BA.guess(gy, h);
+    return Bounder.ARO.qs;
+  }
+}.
+
+(* We want to bound the probability of A winning CPA(Bounder(A,RO),S) in terms of
+   the probability of B = CDH_from_CPA(SCDH_from_CPA(A,RO)) winning CDH(B) *)
 section.
+  declare module A: Adversary {RO, Bounder}.
 
-  declare module A_ : Adversary {RO, ARO, SCDH.SCDH'}.
+  axiom chooseL (O <: ARO {A}): islossless O.o => islossless A(O).choose.
+  axiom guessL (O <: ARO {A}) : islossless O.o => islossless A(O).guess.
 
-  axiom lossless_choose (O <: ARO) : islossless O.o => islossless A_(O).choose.
+  local module BA = Bounder(A,RO).
 
-  axiom lossless_guess (O <: ARO) : islossless O.o => islossless A_(O).guess.
+  local module G0 = {
+    var gxy:group
 
-  local module A = A_(AO).
+    proc main(): bool = {
+      var m0, m1, c, b, b';
+      var x, y, h, gx;
 
-  local module G1 = { 
-    var gxy : group
-
-    fun main() : bool = {
-      var x, y : int;
-      var gx : group;
-      var m0, m1 : plaintext;
-      var c : ciphertext;
-      var b, b' : bool;
-      var h, z : bitstring;   
-      AO.init();
+      H.init();
       x       = $[0..q-1];
       y       = $[0..q-1];
       gx      = g ^ x; 
       gxy     = gx ^ y;
-      (m0,m1) = A.choose(gx);
+      (m0,m1) = BA.choose(gx);
       b       = ${0,1};
-      h       = $uniform;
+      h       = H.hash(gxy);
       c       = (g ^ y, h ^^ (b ? m1 : m0));
-      b'      = A.guess(c);
+      b'      = BA.guess(c);
       return (b' = b);
     }
   }.
 
-  local equiv CPA_G1 :
-    CPA(S, A).main ~ G1.main : true ==> !(mem G1.gxy ARO.log){2} => ={res}.
+  local equiv CPA_G0: CPA(S,BA).main ~ G0.main: ={glob A} ==> ={res}.
   proof.
-    fun.
-    inline AO.init RO.init H.init Hashed_ElGamal(H).kg Hashed_ElGamal(H).enc.
-    swap{1} 9 -5.
-    seq 5 6 : 
-      (={ARO.log, RO.m, y} /\
-       RO.m{1} = FMap.Core.empty /\ ARO.log{2} = FSet.empty /\
-       pk{1} = gx{2} /\ (G1.gxy = gx ^ y){2}); first by wp; do rnd; wp.
-    seq 2 2 : 
-      (={glob A, ARO.log, RO.m, y, b, m0, m1} /\
-       pk{1} = gx{2} /\ (G1.gxy = gx ^ y){2} /\
-       (forall x, mem x ARO.log <=> in_dom x RO.m){2}).   
-      rnd.
-      call (_ : ={RO.m, ARO.log} /\ (forall x, mem x ARO.log <=> in_dom x RO.m){2}).
-        fun; inline RO.o; wp; if; first by smt.
-          by wp; rnd; wp; skip; progress; smt.
-          by wp.
-      by skip; smt.
+    proc.
+    inline Hashed_ElGamal(H).kg Hashed_ElGamal(H).enc.
+    swap{1} 8 -5.
+    call (_: ={glob H, Bounder.ARO.qs}); first by sim.
+    wp; call (_: ={glob H}); first by sim.
+    wp; rnd.
+    call (_: ={glob H, Bounder.ARO.qs}); first by sim.
+    wp; do !rnd.
+    by call (_: true ==> ={glob H}); first by sim.
+  qed.
 
-      call (_ : (mem G1.gxy ARO.log), 
-                (={ARO.log} /\ eq_except RO.m{1} RO.m{2} G1.gxy{2})) => //.
-        by intros O; apply (lossless_guess O).
-   
-        fun; inline RO.o; wp; if; first smt.
-        wp; rnd; wp; skip; progress=> //; first 5 last; last 6 smt.
-        by case (x = G1.gxy){2}; smt.
-        by wp.
-       
-        intros _ _; fun; if; inline RO.o; wp.
-        by rnd; wp; skip; smt.
-        by wp.
-        
-        intros _; fun; if; inline RO.o; wp.
-        by rnd; wp; skip; smt.
-        by wp.
+  local lemma Pr_CPA_G0 &m:
+    Pr[CPA(S,BA).main() @ &m: res] = Pr[G0.main() @ &m: res]
+  by byequiv CPA_G0.
 
-      by inline H.hash RO.o; wp; rnd; wp; skip; progress; smt.
+  local module G1 = { 
+    var gxy : group
+
+    proc main() : bool = {
+      var m0, m1, c, b, b';
+      var x, y, h, gx;
+
+      H.init();
+      x       = $[0..q-1];
+      y       = $[0..q-1];
+      gx      = g ^ x; 
+      gxy     = gx ^ y;
+      (m0,m1) = BA.choose(gx);
+      b       = ${0,1};
+      h       = $uniform;
+      c       = (g ^ y, h ^^ (b ? m1 : m0));
+      b'      = BA.guess(c);
+      return (b' = b);
+    }
+  }.
+
+  local equiv G0_G1:
+    G0.main ~ G1.main: ={glob A} ==> !(mem G1.gxy Bounder.ARO.qs){2} => ={res}.
+  proof.
+    proc.
+    seq  7  7: (={glob BA, x, y, b, m0, m1} /\ G0.gxy{1} = G1.gxy{2} /\
+                (Bounder.ARO.qs = dom RO.m){2}).
+      rnd; call (_: ={glob Bounder, glob H} /\
+                    (Bounder.ARO.qs = dom RO.m){2}).
+        by proc; sp; if=> //; inline RO.o; wp; rnd; wp; skip; smt.
+      by inline H.init RO.init; wp; do !rnd; wp; skip; smt.
+    call (_: (!mem G1.gxy Bounder.ARO.qs){2}
+            => ={glob A, Bounder.ARO.qs, c}
+            /\ eq_except RO.m{1} RO.m{2} G1.gxy{2}
+           ==> (!mem G1.gxy Bounder.ARO.qs){2}
+            => ={glob A, Bounder.ARO.qs, res}
+            /\ eq_except RO.m{1} RO.m{2} G1.gxy{2})=> //.
+      proc (mem G1.gxy Bounder.ARO.qs) (={Bounder.ARO.qs} /\ eq_except RO.m{1} RO.m{2} G1.gxy{2})=> //.
+        smt.
+        smt.
+        by apply guessL.
+        proc; sp; if=> //.
+        inline RO.o; wp; rnd; wp; skip; progress.
+          smt.
+          rewrite eq_except_def=> x' neq.
+          by move: H0; rewrite eq_except_def=> H0; cut:= H0 x' _=> //; smt.
+          smt.
+          by cut:= H0; rewrite eq_except_def; smt.
+          smt.
+          by cut:= H0; rewrite eq_except_def; smt.
+          smt.
+        by progress; proc; sp; if=> //; wp; call (lossless_o _); first smt.
+        progress; proc; sp; if=> //; wp; call (lossless_o _); first smt.
+        by skip; smt.
+    by inline H.hash RO.o; auto; progress; smt.
+  qed.
+
+  local lemma Pr_G0_G1 &m:
+    Pr[G0.main() @ &m: res] <= Pr[G1.main() @ &m: res] + Pr[G1.main() @ &m: mem G1.gxy Bounder.ARO.qs].
+  proof.
+    cut: Pr[G0.main() @ &m: res] <= Pr[G1.main() @ &m: res \/ mem G1.gxy Bounder.ARO.qs].
+      by byequiv G0_G1=> //; smt.
+    by rewrite Pr [mu_or]; smt.
   qed.
 
   local module G2 = {
     var gxy : group
    
-    fun main() : bool = {
-      var x, y : int;
-      var gx : group;
-      var m0, m1 : plaintext;
-      var c : ciphertext;
-      var b, b' : bool;
-      var h, z : bitstring;
-      AO.init();
+    proc main() : bool = {
+      var m0, m1, c, b, b';
+      var x, y, h, gx;
+
+      H.init();
       x        = $[0..q-1];
       y        = $[0..q-1];
       gx       = g ^ x; 
       gxy      = gx ^ y;
-      (m0,m1)  = A.choose(gx);
+      (m0,m1)  = BA.choose(gx);
       h        = $uniform;
       c        = (g ^ y, h);
-      b'       = A.guess(c);
+      b'       = BA.guess(c);
       b        = ${0,1};
       return (b' = b);
     }
   }.
-   
-   
-  local equiv G1_G2 :
-     G1.main ~ G2.main : true ==> ={res, ARO.log} /\ G1.gxy{1} = G2.gxy{2}.
+
+  local equiv G1_G2:
+     G1.main ~ G2.main: ={glob A} ==> ={res, Bounder.ARO.qs} /\ G1.gxy{1} = G2.gxy{2}.
   proof.
-    fun.
-    inline AO.init RO.init.
-    swap{2} 11 -3.
-    call (_ : ={ARO.log, RO.m} /\ G1.gxy{1} = G2.gxy{2}).
-      fun; inline RO.o; wp; if; first smt.
-        by wp; rnd; wp; skip; smt.
-        by wp.
+    proc.
+    swap{2} 10 -3.
+    call (_: ={glob H} /\ G1.gxy{1} = G2.gxy{2});
+      first by sim.
     wp.
-    rnd (lambda h, h ^^ if b then m1 else m0){1}; rnd.
-    call ( _ : ={ARO.log, RO.m} /\ G1.gxy{1} = G2.gxy{2}).
-    fun; inline RO.o; wp; if; first smt.
-      by wp; rnd; wp; skip; smt.
-      by wp.
-    wp; do rnd; wp; skip; progress=> //; smt.
+    rnd (fun h, h ^^ if b then m1 else m0){1}; rnd.
+    call (_: ={glob H} /\ G1.gxy{1} = G2.gxy{2}).
+      by sim.
+    inline H.init RO.init.
+    auto; progress; first 2 smt.
+      by rewrite /(^^) /(^^) -xorwA xorwK xorw0.
+      by rewrite /(^^) /(^^) -xorwA xorwK xorw0.
   qed.
-   
-  local module SCDH_from_CPA : SCDH.Adversary = {
-    fun solve(gx:group, gy:group) : group set = {
-      var m0, m1 : plaintext;
-      var h : bitstring;
-      var b' : bool;
-      AO.init();
-      (m0,m1)  = A.choose(gx);
-      h        = $uniform;
-      b'       = A.guess((gy, h));
-      return ARO.log;
-    }
-  }.
-   
-  local equiv G2_SCDH :
-    G2.main ~ SCDH.SCDH(SCDH_from_CPA).main : 
-    true ==> (mem G2.gxy ARO.log){1} = res{2} /\ card ARO.log{1} <= qH.
+
+  local lemma Pr_G1_G2_res &m:
+    Pr[G1.main() @ &m: res] = Pr[G2.main() @ &m: res]
+  by byequiv G1_G2.
+
+  local lemma Pr_G1_G2_coll &m:
+    Pr[G1.main() @ &m: mem G1.gxy Bounder.ARO.qs] = Pr[G2.main() @ &m: mem G2.gxy Bounder.ARO.qs]
+  by byequiv G1_G2.
+
+  local lemma Pr_G2 &m: Pr[G2.main() @ &m: res] = 1%r / 2%r.
   proof.
-    fun.
-    inline SCDH_from_CPA.solve AO.init RO.init.
-    swap{2} [5..6] -4.  
-    rnd{1}; wp.  
-    seq 9 8 : 
-      ((glob A){1} = (glob A){2} /\ ={ARO.log, RO.m} /\
-      c{1} = (gy, h){2} /\ G2.gxy{1} = g ^ (x * y){2} /\ card ARO.log{1} <= qH).
-      wp; rnd; call ( _ : ={ARO.log, RO.m} /\ card ARO.log{1} <= qH).
-      fun; inline RO.o; wp; if; first by smt.
-        by wp; rnd; wp; skip; smt.
-        by wp.
-      by wp; do rnd; wp; skip; smt.
-   
-      call ( _ :
-       RO.m{1} = RO.m{2} /\ ARO.log{1} = ARO.log{2} /\ card ARO.log{1} <= qH).
-        fun; inline RO.o; wp; if; first smt.
-          by wp; rnd; wp; skip; smt.
-          by wp.
-        by skip; smt.
-  qed.
-      
-  local lemma Pr_CPA_G1 &m :
-    Pr[CPA(S, A).main() @ &m : res] <=
-    Pr[G1.main() @ &m : res \/ mem G1.gxy ARO.log]. 
-  proof.
-    by equiv_deno CPA_G1 => //; smt.
-  qed.
-      
-  local lemma Pr_G1_G1 &m :
-    Pr[G1.main() @ &m : res \/ mem G1.gxy ARO.log] <=
-    Pr[G1.main() @ &m : res] + Pr[G1.main() @ &m : mem G1.gxy ARO.log].
-  proof.
-    apply (Trans _
-      (Pr[G1.main() @ &m : res] + 
-       Pr[G1.main() @ &m : mem G1.gxy ARO.log] -
-       Pr[G1.main() @ &m : res /\ mem G1.gxy ARO.log])).
-    cut W: (forall (x y:real), x = y => x <= y) by smt.
-    by apply W; rewrite Pr mu_or; smt.
-    by smt.
-  qed.
-   
-  local lemma Pr_G1_G2_res &m : 
-    Pr[G1.main() @ &m : res] = Pr[G2.main() @ &m : res].
-  proof.
-    by equiv_deno G1_G2=> //; smt.
-  qed.
-      
-  local lemma Pr_G1_G2_mem &m : 
-    Pr[G1.main() @ &m : mem G1.gxy ARO.log] = 
-    Pr[G2.main() @ &m : mem G2.gxy ARO.log].
-  proof.
-    by equiv_deno G1_G2=> //; smt.
-  qed.
-  
-  local lemma Pr_G2 &m : Pr[G2.main() @ &m : res] = 1%r / 2%r.
-  proof.
-    bdhoare_deno (_ : true ==> _) => //.
-    fun; rnd ((=) b').
-    call (_ : true) => //.
-    by intros => O _; apply (lossless_guess O).
-    by apply RO_lossless_o; smt.
+    byphoare (_: true ==> _)=> //.
+    proc; rnd ((=) b').
+    call (_: true)=> //.
+      by apply guessL.
+      by proc; sp; if=> //; wp; call (lossless_o _); first smt.
     wp; rnd; call (_ : true).
-    by intros => O _; apply (lossless_choose O).
-    by apply RO_lossless_o; smt.
-    by wp; do rnd; inline AO.init RO.init; wp; skip; progress; smt.
+      by apply chooseL.
+      by proc; sp; if=> //; wp; call (lossless_o _); first smt.
+    by inline H.init RO.init; auto; progress; smt.
+  qed.
+
+  local equiv G2_SCDH: G2.main ~ SCDH.SCDH(SCDH_from_CPA(A,RO)).main:
+    ={glob A} ==> (mem G2.gxy Bounder.ARO.qs){1} = res{2} /\ card Bounder.ARO.qs{1} <= qH.
+  proof.
+    proc.
+    inline SCDH_from_CPA(A,RO).solve.
+    swap{2} 5 -4.
+    rnd{1}; wp.  
+    seq  8  7: (={glob BA} /\
+                c{1} = (gy, h){2} /\
+                G2.gxy{1} = g ^ (x * y){2} /\
+                card Bounder.ARO.qs{1} <= qH).
+      wp; rnd; call (_: ={glob H} /\ card Bounder.ARO.qs{1} <= qH).
+        by proc; sp; if=> //; inline RO.o; auto; smt.
+      by inline H.init RO.init; auto; smt.
+    call (_: ={glob H} /\ card Bounder.ARO.qs{1} <= qH).
+      by proc; sp; if=> //; inline RO.o; auto; smt.
+    by skip; smt.
   qed.
       
   local lemma Pr_G2_SCDH &m : 
-    Pr[G2.main() @ &m : mem G2.gxy ARO.log] =
-    Pr[SCDH.SCDH(SCDH_from_CPA).main() @ &m : res].
-  proof.
-    by equiv_deno G2_SCDH.
-  qed.
+    Pr[G2.main() @ &m : mem G2.gxy Bounder.ARO.qs]
+    = Pr[SCDH.SCDH(SCDH_from_CPA(A,RO)).main() @ &m : res]
+  by byequiv G2_SCDH.
    
   local lemma Reduction &m :
-    Pr[CPA(S, A).main() @ &m : res] <=
-    1%r / 2%r + Pr[SCDH.SCDH(SCDH_from_CPA).main() @ &m : res].
+    Pr[CPA(S,BA).main() @ &m : res] <=
+    1%r / 2%r + Pr[SCDH.SCDH(SCDH_from_CPA(A,RO)).main() @ &m : res].
   proof. 
-    apply (Trans _ Pr[G1.main() @ &m : res \/ mem G1.gxy ARO.log]);
-    first by apply (Pr_CPA_G1 &m).
-    apply (Trans _
-      (Pr[G1.main() @ &m : res] + Pr[G1.main() @ &m : mem G1.gxy ARO.log])).
-    by apply (Pr_G1_G1 &m).
-    by rewrite (Pr_G1_G2_res &m) (Pr_G2 &m) (Pr_G1_G2_mem &m) (Pr_G2_SCDH &m).
+    rewrite (Pr_CPA_G0 &m).
+    apply (Trans _ (Pr[G1.main() @ &m : res] + Pr[G1.main() @ &m: mem G1.gxy Bounder.ARO.qs]));
+      first by apply (Pr_G0_G1 &m).
+    by rewrite (Pr_G1_G2_res &m) (Pr_G2 &m) (Pr_G1_G2_coll &m) (Pr_G2_SCDH &m).
   qed.
-   
-  local lemma Security_SCDH &m :
-    exists (B <: SCDH.Adversary {SCDH.SCDH'}),
-      Pr[CPA(S, A).main() @ &m : res] - 1%r / 2%r <= 
-      Pr[SCDH.SCDH(B).main() @ &m : res].
-  proof.
-    exists SCDH_from_CPA.
-    cut W : forall (x y z : real), x <= z + y => x - z <= y by smt.
-    by apply W; apply (Reduction &m).
-  qed.
-   
+
   lemma mult_inv_le_r (x y z:real) : 
     0%r < x => (1%r / x) * y <= z => y <= x * z
   by [].
 
   (** Composing reduction from CPA to SCDH with reduction from SCDH to CDH *)
   lemma Security &m :
-    exists (B <: CDH.Adversary),
-      Pr[CPA(S, A_(AO)).main() @ &m : res] - 1%r / 2%r <= 
-      qH%r * Pr[CDH.CDH(B).main() @ &m : res].
+      Pr[CPA(S,Bounder(A,RO)).main() @ &m: res] - 1%r / 2%r <= 
+      qH%r * Pr[CDH.CDH(SCDH.CDH_from_SCDH(SCDH_from_CPA(A,RO))).main() @ &m: res].
   proof.
-    elim (Security_SCDH &m) => B H.
-    elim (SCDH.Reduction B &m _); first by smt.
-    intros C H1; exists C.
-    apply (Trans _ Pr[SCDH.SCDH(B).main() @ &m : res]) => //.
-    by apply mult_inv_le_r; first smt.
+    apply (Trans _ (Pr[SCDH.SCDH(SCDH_from_CPA(A,RO)).main() @ &m: res]));
+      first smt.
+    apply mult_inv_le_r; first smt.
+    by apply (SCDH.Reduction (SCDH_from_CPA(A,RO)) &m); smt.
   qed.
-     
-  lemma Correctness : 
-    hoare [Correctness(S).main : true ==> res].
-  proof.
-    fun.
-    inline Hashed_ElGamal(H).kg Hashed_ElGamal(H).enc Hashed_ElGamal(H).dec.
-    inline H.hash RO.o H.init AO.init RO.init.
-    by do (wp; rnd); wp; skip; progress; smt.
-  qed.
-
 end section.
 
 print axiom Security.
